[svl] improvements in simplify-bitand-or-xor.lisp. Now repeated args in bitxor, bitor, bitand in nested calls are cleared more successfully.

books/centaur/svl/svex-reduce/simplify-bitand-or-xor.lisp
@@ -34,6 +34,7 @@
 
 (include-book "svex-reduce-apply")
 (include-book "integerp-of-svex")
+(include-book "width-of-svex")
 
 (local
  (include-book "../4vec-lemmas"))
@@ -45,13 +46,13 @@
  (rp::fetch-new-events
   (include-book "centaur/bitops/ihs-extensions" :dir :system)
   use-ihs-extensions
-  :disabled t))
+  ))
 
 (local
  (rp::fetch-new-events
   (include-book "ihs/logops-lemmas" :dir :system)
   use-ihs-logops-lemmas
-  :disabled t))
+  ))
 
 (local
  (rp::fetch-new-events
@@ -63,7 +64,7 @@
  (rp::fetch-new-events
   (include-book "ihs/quotient-remainder-lemmas" :dir :system)
   use-qr-lemmas
-  :disabled t))
+  ))
 
 (local
  (rp::fetch-new-events
@@ -81,221 +82,380 @@
    :hints (("Goal"
             :in-theory (e/d (svex-p) ())))))
 
-(acl2::defsection bitand/bitor-cancel-repeated
-  (define bitand/bitor-collect-leaves ((svex)
-                                       (fn))
-    :Returns (leaves sv::Svexlist-p :hyp (and (sv::Svex-p svex)
-                                              (not (equal fn ':var)))
-                     :hints (("Goal"
-                              :in-theory (e/d (svex-p
-                                               4vec-p)
-                                              ()))))
-    (case-match svex
-      ((this-fn x y)
-       (if (equal this-fn fn)
-           (cons svex (append (bitand/bitor-collect-leaves x fn)
-                              (bitand/bitor-collect-leaves y fn)))
-         (list svex)))
-      (& (list svex)))
-    ///
-    (defret true-listp-of-<fn>
-      (true-listp leaves)))
+(local
+ (defthm svex-p-of-4vec-p
+   (implies (4vec-p x)
+            (svex-p x))
+   :rule-classes :rewrite
+   :hints (("Goal"
+            :in-theory (e/d (svex-p 4vec-p) ())))))
 
-  (define bitand/or/xor-simple-constant-simplify (fn arg1 arg2 &optional 1masked)
-    ;; for easier theorem proving,
-    :returns (simplified-svex sv::Svex-p :hyp (and (sv::fnsym-p fn)
-                                                   (not (equal fn ':var))
-                                                   (sv::Svex-p arg1)
-                                                   (sv::Svex-p arg2)))
-    (cond ((equal fn 'sv::bitor)
-           (b* (((when (and 1masked
-                            (or (equal arg1 1)
-                                (equal arg2 1))))
-                 1)
-                ((when (and (not 1masked)
-                            (or (equal arg1 -1)
-                                (equal arg2 -1))))
-                 -1)
-                ((when (equal arg1 0))
-                 (svex-reduce-w/-env-apply 'sv::unfloat (hons-list arg2)))
-                ((when (equal arg2 0))
-                 (svex-reduce-w/-env-apply 'sv::unfloat (hons-list arg1))))
-             (svex-reduce-w/-env-apply 'sv::bitor (hons-list arg1 arg2))))
-          ((equal fn 'sv::bitxor)
-           (b* (((when (equal arg1 0))
-                 (svex-reduce-w/-env-apply 'sv::unfloat (hons-list arg2)))
-                ((when (equal arg2 0))
-                 (svex-reduce-w/-env-apply 'sv::unfloat (hons-list arg1))))
-             (svex-reduce-w/-env-apply 'sv::bitxor (hons-list arg1 arg2))))
-          ((equal fn 'sv::bitand)
-           (b*  (((when (or (equal arg1 0)
-                            (equal arg2 0)))
-                  0)
-                 ((when (or (equal arg1 -1)
-                            (and 1masked (equal arg1 1))))
-                  (svex-reduce-w/-env-apply 'sv::unfloat (hons-list arg2)))
-                 ((when (or (equal arg2 -1)
-                            (and 1masked (equal arg2 1))))
-                  (svex-reduce-w/-env-apply 'sv::unfloat (hons-list arg1))))
-             (svex-reduce-w/-env-apply 'sv::bitand (hons-list arg1 arg2))))
-          (t (svex-reduce-w/-env-apply fn (hons-list arg1 arg2)))))
+(define bitand/or/xor-simple-constant-simplify (fn (arg1 svex-p)
+                                                   (arg2 svex-p)
+                                                   &optional 1masked)
+  ;; for easier theorem proving,
+  :returns (simplified-svex sv::Svex-p :hyp (and (sv::fnsym-p fn)
+                                                 (not (equal fn ':var))
+                                                 (sv::Svex-p arg1)
+                                                 (sv::Svex-p arg2)))
+  (cond ((equal fn 'sv::bitor)
+         (b* (((when (and* (4vec-p arg1)
+                           (4vec-p arg2)))
+               (4vec-bitor arg1 arg2))
+              ((when (and 1masked
+                          (or (equal arg1 1)
+                              (equal arg2 1))))
+               1)
+              ((when (and (not 1masked) ;; not necessarry
+                          (or (equal arg1 -1)
+                              (equal arg2 -1))))
+               -1)
 
-  (define member-hons-equal (x lst)
-    (if (atom lst)
-        nil
-      (or (hons-equal x (car lst))
-          (member-hons-equal x (cdr lst))))
-    ///
-    (defthm member-hons-equal-is-member-equal
-      (iff (member-hons-equal x lst)
-           (member-equal x lst))))
+              ((when (and (not 1masked) ;; not necessary
+                          (or (and (equal arg1 1)
+                                   (let* ((arg2-width (width-of-svex arg2)))
+                                     (and arg2-width
+                                          (equal arg2-width 1))))
+                              (and (equal arg2 1)
+                                   (let* ((arg1-width (width-of-svex arg1)))
+                                     (and arg1-width
+                                          (equal arg1-width 1)))))))
+               1)
 
-  (defconst *bitand/bitor-cancel-repeated-aux-limit*
-    5)
+              ((when (equal arg1 0))
+               (svex-reduce-w/-env-apply 'sv::unfloat (hons-list arg2)))
+              ((when (equal arg2 0))
+               (svex-reduce-w/-env-apply 'sv::unfloat (hons-list arg1))))
+           (svex-reduce-w/-env-apply 'sv::bitor (hons-list arg1 arg2))))
+        ((equal fn 'sv::bitxor)
+         (b* (((when (equal arg1 0))
+               (svex-reduce-w/-env-apply 'sv::unfloat (hons-list arg2)))
+              ((when (equal arg2 0))
+               (svex-reduce-w/-env-apply 'sv::unfloat (hons-list arg1))))
+           (svex-reduce-w/-env-apply 'sv::bitxor (hons-list arg1 arg2))))
+        ((equal fn 'sv::bitand)
+         (b*  (((when (or (equal arg1 0)
+                          (equal arg2 0)))
+                0)
+               ((when (or (equal arg1 -1)
+                          (and (equal arg1 1)
+                               (or 1masked
+                                   (let* ((arg2-width (width-of-svex arg2)))
+                                     (and arg2-width
+                                          (equal arg2-width 1)))))))
+                (svex-reduce-w/-env-apply 'sv::unfloat (hons-list arg2)))
+               ((when (or (equal arg2 -1)
+                          (and (equal arg2 1)
+                               (or 1masked
+                                   (let* ((arg1-width (width-of-svex arg1)))
+                                     (and arg1-width
+                                          (equal arg1-width 1)))))))
+                (svex-reduce-w/-env-apply 'sv::unfloat (hons-list arg1))))
+           (svex-reduce-w/-env-apply 'sv::bitand (hons-list arg1 arg2))))
+        (t (svex-reduce-w/-env-apply fn (hons-list arg1 arg2)))))
 
-  (define bitand/bitor-cancel-repeated-aux ((svex sv::svex-p)
-                                            (leaves svexlist-p)
-                                            (new-val integerp)
-                                            &key
-                                            (1masked '1masked)
-                                            ((limit natp) '*bitand/bitor-cancel-repeated-aux-limit*)
-                                            ;;((require-integerp booleanp) 'require-integerp)
-                                            ((env) 'env)
-                                            ((context rp::rp-term-listp) 'context))
-    :verify-guards nil
-    :returns (mv (simplified-svex sv::svex-p
-                                  :hyp (and (sv::svex-p svex)
-                                            (sv::Svex-p new-val))
-                                  :hints (("Goal"
-                                           :in-theory (e/d (sv::Svex-p) ()))))
-                 changed)
-    (cond
-     ((zp limit)
-      (mv svex nil))
-     ((member-hons-equal svex leaves)
-      (mv new-val t))
-     ((and (consp svex)
-           (equal (car svex) 'sv::Bitor)
-           (equal-len (cdr svex) 2))
-      (b* ((x (first (cdr svex))) (y (second (cdr svex)))
-           ((mv x changed-x) (bitand/bitor-cancel-repeated-aux x leaves new-val :limit (1- limit)))
-           ((mv y changed-y) (bitand/bitor-cancel-repeated-aux y leaves new-val :limit (1- limit))))
-        (if (or changed-x
-                changed-y)
-            (mv (bitand/or/xor-simple-constant-simplify 'sv::bitor x y 1masked) t)
-          (mv svex nil))))
-     ((and (consp svex)
-           (equal (car svex) 'sv::bitand)
-           (equal-len (cdr svex) 2))
-      (b* ((x (first (cdr svex))) (y (second (cdr svex)))
-           ((mv x changed-x) (bitand/bitor-cancel-repeated-aux x leaves new-val :limit (1- limit)))
-           ((mv y changed-y) (bitand/bitor-cancel-repeated-aux y leaves new-val :limit (1- limit))))
-        (if (or changed-x
-                changed-y)
-            (mv (bitand/or/xor-simple-constant-simplify 'sv::bitand x y 1masked) t)
-          (mv svex nil))))
-     ((and (consp svex)
-           (equal (car svex) 'sv::bitxor)
-           (equal-len (cdr svex) 2))
-      (b* ((x (first (cdr svex))) (y (second (cdr svex)))
-           ((mv new-x changed-x) (bitand/bitor-cancel-repeated-aux x leaves new-val :limit (1- limit)))
-           ((mv new-y changed-y) (bitand/bitor-cancel-repeated-aux y leaves new-val :limit (1- limit))))
-        (if (and (or changed-x changed-y)
-                 (integer-listp-of-svexlist leaves))
-            (mv (bitand/or/xor-simple-constant-simplify 'sv::bitxor new-x new-y 1masked) t)
-          (mv svex nil))))
-     (t (mv svex nil))))
+(defsection clear-1s-from-bitxor
+  ;; A quick  way to  clear repeated  1's from bitxors.  These are  expected to
+  ;; appear in bitand/bitor-cancel-repeated
+
+  (define bitxor-has-1 (x)
+    :returns (res)
+    (case-match x
+      (('sv::bitxor a b)
+       (or (equal a 1)
+           (equal b 1)
+           (bitxor-has-1 a)
+           (bitxor-has-1 b)))
+      (& (equal x 1))))
+
+  (define remove-1-from-xor ((x svex-p))
+    :returns (res svex-p :hyp (svex-p x))
+    (case-match x
+      (('sv::bitxor a b)
+       (cond ((equal a 1)
+              (svex-reduce-w/-env-apply 'sv::unfloat (hons-list b)))
+             ((equal b 1)
+              (svex-reduce-w/-env-apply 'sv::unfloat (hons-list a)))
+             ((bitxor-has-1 a)
+              (bitand/or/xor-simple-constant-simplify 'sv::bitxor
+                                                      (remove-1-from-xor a) b))
+             ((bitxor-has-1 b)
+              (bitand/or/xor-simple-constant-simplify 'sv::bitxor
+                                                      a
+                                                      (remove-1-from-xor b)))
+             (t x)
+             ))
+      (& (if (equal x 1) 0 x))))
+
+  (define clear-1s-from-bitxor ((x svex-p))
+    :returns (res svex-p :hyp (svex-p x))
+    (case-match x
+      (('sv::bitxor a b)
+       (b* (((unless (and (bitxor-has-1 a)
+                          (bitxor-has-1 b)))
+             x)
+            (a (remove-1-from-xor a))
+            (b (remove-1-from-xor b)))
+         (bitand/or/xor-simple-constant-simplify 'sv::bitxor a b)))
+      (& x)))
+
+  ;;(clear-1s-from-bitxor `(bitxor (bitxor 1 x) (bitxor (bitxor 1 y) z)))
+  ;; returns:
+  ;; (BITXOR X (BITXOR Y Z))
+  )
+
+(define bitand/or/xor-collect-leaves ((svex)
+                                      (fn))
+  :Returns (leaves sv::Svexlist-p :hyp (and (sv::Svex-p svex)
+                                            (not (equal fn ':var)))
+                   :hints (("Goal"
+                            :in-theory (e/d (svex-p
+                                             4vec-p)
+                                            ()))))
+  (case-match svex
+    ((this-fn x y)
+     (if (equal this-fn fn)
+         (cons svex (append (bitand/or/xor-collect-leaves x fn)
+                            (bitand/or/xor-collect-leaves y fn)))
+       (list svex)))
+    (& (list svex)))
+  ///
+  (defret true-listp-of-<fn>
+    (true-listp leaves)))
+
+(define member-hons-equal (x lst)
+  (if (atom lst)
+      nil
+    (or (hons-equal x (car lst))
+        (member-hons-equal x (cdr lst))))
+  ///
+  (defthm member-hons-equal-is-member-equal
+    (iff (member-hons-equal x lst)
+         (member-equal x lst))))
+
+(define bitand/bitor-cancel-repeated-aux ((svex sv::svex-p)
+                                          (leaves svexlist-p)
+                                          (new-val integerp)
+                                          &key
+                                          (under-xor 'under-xor)
+                                          ((limit natp) '*bitand/bitor-cancel-repeated-aux-limit*)
+                                          ;;((require-integerp booleanp) 'require-integerp)
+                                          ((env) 'env)
+                                          ((context rp::rp-term-listp) 'context))
+  :verify-guards nil
+  :prepwork
+  (
+   ;; TODO: (partial) memoization can help here  to increase the limit. This may
+   ;; require having a very large limit though, which might be bad again.
+   (defconst *bitand/bitor-cancel-repeated-aux-limit*
+     5))
+
+  :returns (mv (simplified-svex sv::svex-p
+                                :hyp (and (sv::svex-p svex)
+                                          (sv::Svex-p new-val))
+                                :hints (("Goal"
+                                         :in-theory (e/d (sv::Svex-p) ()))))
+               changed)
+  (cond
+   ((zp limit)
+    (mv svex nil))
+   ((member-hons-equal svex leaves)
+    (b* (((Unless (and under-xor
+                       (not (equal new-val 0))))
+          (mv new-val t))
+         (width (width-of-svex svex))
+         ((Unless width)
+          (mv new-val t)))
+      (mv (4vec-part-select 0 width new-val) t)))
+   ((and (consp svex)
+         (equal (car svex) 'sv::bitor)
+         (equal-len (cdr svex) 2))
+    (b* ((x (first (cdr svex))) (y (second (cdr svex)))
+         ((mv x changed-x) (bitand/bitor-cancel-repeated-aux x leaves new-val :limit (1- limit)))
+         ((mv y changed-y) (bitand/bitor-cancel-repeated-aux y leaves new-val :limit (1- limit))))
+      (if (or changed-x
+              changed-y)
+          (mv (bitand/or/xor-simple-constant-simplify 'sv::bitor x y nil) t)
+        (mv svex nil))))
+   ((and (consp svex)
+         (equal (car svex) 'sv::bitand)
+         (equal-len (cdr svex) 2))
+    (b* ((x (first (cdr svex))) (y (second (cdr svex)))
+         ((mv x changed-x) (bitand/bitor-cancel-repeated-aux x leaves new-val :limit (1- limit)))
+         ((mv y changed-y) (bitand/bitor-cancel-repeated-aux y leaves new-val :limit (1- limit))))
+      (if (or changed-x
+              changed-y)
+          (mv (bitand/or/xor-simple-constant-simplify 'sv::bitand x y nil) t)
+        (mv svex nil))))
+   ((and (consp svex)
+         (equal (car svex) 'sv::bitxor)
+         (equal-len (cdr svex) 2))
+    (b* ((x (first (cdr svex))) (y (second (cdr svex)))
+         ((mv new-x changed-x) (bitand/bitor-cancel-repeated-aux x leaves new-val :limit (1- limit) :under-xor t))
+         ((mv new-y changed-y) (bitand/bitor-cancel-repeated-aux y leaves new-val :limit (1- limit) :under-xor t))
+         ((Unless (and (or changed-x changed-y)
+                       (integer-listp-of-svexlist leaves)))
+          (mv svex nil))
+         (res (bitand/or/xor-simple-constant-simplify 'sv::bitxor new-x new-y nil))
+         (res (clear-1s-from-bitxor res)))
+      (mv res t)))
+   (t (mv svex nil)))
+
+  ///
 
   (verify-guards bitand/bitor-cancel-repeated-aux-fn
     :hints (("Goal"
              :do-not-induct t
-             :in-theory (e/d (SVEX-P) ()))))
+             :in-theory (e/d (SVEX-P) ())))))
 
-  (define bitand/bitor-cancel-repeated (fn
-                                        (x sv::svex-p)
-                                        (y sv::svex-p)
-                                        &key
-                                        (1masked 'nil)
-                                        ((env) 'env)
-                                        ((context rp::rp-term-listp) 'context))
+(defsection bitxor-cancel-repeated-aux-functions
+  ;; TODO: Maybe a limit should be imposed for cancelling repeated in bitxor...
 
-    :returns (simplified-svex sv::Svex-p :hyp (and (sv::fnsym-p fn)
-                                                   (Not (equal fn :var))
-                                                   (svex-p x)
-                                                   (svex-p y)))
-    (case fn
-      (sv::bitor
-       (b* (;;(require-integerp nil)
-            (l1
-             (bitand/bitor-collect-leaves x 'sv::bitor))
-            ((mv y changed-y) (bitand/bitor-cancel-repeated-aux y l1 0))
-            (l2
-             (bitand/bitor-collect-leaves y 'sv::bitor))
-            ((mv x changed-x) (bitand/bitor-cancel-repeated-aux x l2  0)))
-         (if (or changed-x changed-y)
-             (bitand/or/xor-simple-constant-simplify 'sv::bitor x y nil)
-           (svex-reduce-w/-env-apply fn (hons-list x y)))))
-      (sv::bitand
-       (b* (;;(require-integerp nil)
-            (l1
-             (bitand/bitor-collect-leaves x 'sv::bitand))
-            ((mv y changed-y) (bitand/bitor-cancel-repeated-aux y l1  (if 1masked 1 -1)))
-            (l2
-             (bitand/bitor-collect-leaves y 'sv::bitand))
-            ((mv x changed-x) (bitand/bitor-cancel-repeated-aux x l2  (if 1masked 1 -1))))
-         (if (or changed-x changed-y)
-             (bitand/or/xor-simple-constant-simplify 'sv::bitand x y nil)
-           (svex-reduce-w/-env-apply fn (hons-list x y)))))
-      (otherwise
-       (svex-reduce-w/-env-apply fn (hons-list x y)))))
+  (defconst *bitxor-cancel-repeated-limit*
+    3)
+  
+  (define bitxor-collect-repeated (svex leaves (limit natp))
+    :Returns (commons sv::Svexlist-p :hyp (and (sv::Svex-p svex))
+                      :hints (("Goal"
+                               :in-theory (e/d (svex-p
+                                                4vec-p)
+                                               ()))))
+    ;; Using the leaves from the other arg of bitxor, find the commons.
+    (cond
+     ((zp limit)
+      nil)
+     ((member-hons-equal svex leaves)
+      (and ;;(not (4vec-p svex)) ;; don't clear constants as they likely come from bitnot.
+           (list svex)))
+     (t 
+      (case-match svex
+        (('bitxor x y)
+         (append (bitxor-collect-repeated x leaves (1- limit))
+                 (bitxor-collect-repeated y leaves (1- limit))))))))
 
-  ;; (bitand/bitor-cancel-repeated '(sv::Bitand (sv::Bitand a b)
-  ;;                                            (sv::bitand (sv::bitor a x) y)))
-  ;; returns:
-  ;; (BITAND (BITAND A B) Y)
+  (define bitxor-remove-node ((svex svex-p)
+                              (node-to-remove)
+                              (limit natp))
+    :returns (mv (res-svex svex-p :hyp (svex-p svex))
+                 success)
+    ;; try to remove a node from an svex.
+    :verify-guards :after-returns
+    (cond
+     ((zp limit)
+      (mv svex nil))
+     ((hons-equal svex node-to-remove)
+      (mv 0 t))
+     (t 
+      (case-match svex
+        (('bitxor x y)
+         (b* (((mv new-x success-x)
+               (bitxor-remove-node x node-to-remove (1- limit)))
+              ((when success-x) ;; allowed to be replaced only once.
+               (mv (bitand/or/xor-simple-constant-simplify 'sv::bitxor new-x y nil) t))
+              ((mv new-y success-y)
+               (bitxor-remove-node y node-to-remove (1- limit))))
+           (if success-y
+               (mv (bitand/or/xor-simple-constant-simplify 'sv::bitxor x new-y nil) t)
+             (mv svex nil))))
+        (& (mv svex nil))))))
 
-  ;; (bitand/bitor-cancel-repeated '(sv::Bitor (sv::Bitor a b)
-  ;;                                           (sv::bitand (sv::bitor a x) y)))
-  ;; returns:
-  ;; (SV::BITOR (SV::BITOR A B) (BITAND X Y))
+  (define bitxor-remove-nodes-from-both ((svex1 svex-p)
+                                         (svex2 svex-p)
+                                         (nodes-to-remove svexlist-p)
+                                         &optional
+                                         ((env) 'env)
+                                         ((context rp::rp-term-listp) 'context))
+    :returns (mv (res-svex1 svex-p :hyp (svex-p svex1))
+                 (res-svex2 svex-p :hyp (svex-p svex2)))
+    ;; Try removing from both svexes at the same time.
+    (if (atom nodes-to-remove)
+        (mv svex1 svex2)
+      (b* ((limit *bitxor-cancel-repeated-limit*)
+           ((mv new-svex1 success-1)
+            (bitxor-remove-node svex1 (car nodes-to-remove) limit))
+           ((Unless success-1) ;; expected to never happen
+            (bitxor-remove-nodes-from-both svex1 svex2 (cdr nodes-to-remove)))
+           ((mv new-svex2 success-2)
+            (bitxor-remove-node svex2 (car nodes-to-remove) limit))
+           ((Unless success-2) ;; expected to never happen
+            (bitxor-remove-nodes-from-both svex1 svex2 (cdr nodes-to-remove)))
+           ((unless (integerp-of-svex (car nodes-to-remove)))
+            (bitxor-remove-nodes-from-both svex1 svex2 (cdr nodes-to-remove))))
 
-  ;; (bitand/bitor-cancel-repeated '(sv::Bitor a (sv::bitxor 1 a)))
-  ;; returns:
-  ;; 1
+        (bitxor-remove-nodes-from-both new-svex1 new-svex2 (cdr nodes-to-remove))))))
 
-  ;; (bitand/bitor-cancel-repeated 'sv::bitand `x `(sv::bitxor x y)
-  ;;                               :env (make-fast-alist `((x . x) (y . y)))
-  ;;                               :context `((integerp x) (Integerp y)))
-  ;; returns
-  ;; (BITAND X (BITXOR -1 Y))
-  )
+(define bitand/or/xor-cancel-repeated (fn
+                                       (x sv::svex-p)
+                                       (y sv::svex-p)
+                                       &key
+                                       ((env) 'env)
+                                       ((context rp::rp-term-listp) 'context))
 
-(define all-xor/and/or-nodes-are-masked-p (svex size env)
-  :verify-guards nil
-  :returns res
-  (and (let* ((x (svex-eval svex env)))
-         (equal (4vec-part-select 0 size x) x))
+  :returns (simplified-svex sv::Svex-p :hyp (and (sv::fnsym-p fn)
+                                                 (Not (equal fn :var))
+                                                 (svex-p x)
+                                                 (svex-p y)))
+  (case fn
+    (sv::bitor
+     (b* ((under-xor nil)
+          (l1 (bitand/or/xor-collect-leaves x 'sv::bitor))
+          ((mv y changed-y) (bitand/bitor-cancel-repeated-aux y l1 0))
+          (l2 (bitand/or/xor-collect-leaves y 'sv::bitor))
+          ((mv x changed-x) (bitand/bitor-cancel-repeated-aux x l2  0)))
+       (if (or changed-x changed-y)
+           (bitand/or/xor-simple-constant-simplify 'sv::bitor x y nil)
+         (svex-reduce-w/-env-apply fn (hons-list x y)))))
+    (sv::bitand
+     (b* ((under-xor nil)
+          (l1 (bitand/or/xor-collect-leaves x 'sv::bitand))
+          ((mv y changed-y) (bitand/bitor-cancel-repeated-aux y l1  -1))
+          (l2 (bitand/or/xor-collect-leaves y 'sv::bitand))
+          ((mv x changed-x) (bitand/bitor-cancel-repeated-aux x l2  -1)))
+       (if (or changed-x changed-y)
+           (bitand/or/xor-simple-constant-simplify 'sv::bitand x y nil)
+         (svex-reduce-w/-env-apply fn (hons-list x y)))))
+    (sv::bitxor
+     (b* ((limit *bitxor-cancel-repeated-limit*)
+          (leaves (bitand/or/xor-collect-leaves x 'sv::bitxor))
+          (commons (bitxor-collect-repeated y leaves limit))
+          (- (and commons
+                  (rp::cwe "Some commons in botxor are found: ~p0 in x:~p1 and y:~p2~%" commons x y)))
+          ((mv x y) (bitxor-remove-nodes-from-both x y commons)))
+       (svex-reduce-w/-env-apply fn (hons-list x y))))
+    (otherwise
+     (svex-reduce-w/-env-apply fn (hons-list x y)))))
 
-       (cond
-        ((acl2::and* (consp svex)
-                     (equal-len (cdr svex) 2)
-                     (or (equal (car svex) 'sv::bitand)
-                         (equal (car svex) 'sv::bitor)
-                         (equal (car svex) 'sv::bitxor)))
-         (b* ((res1 (all-xor/and/or-nodes-are-masked-p (first (cdr svex)) size env))
-              (res2 (all-xor/and/or-nodes-are-masked-p (second (cdr svex)) size env)))
-           (and res1 res2)))
-        ((acl2::and* (consp svex)
-                     (equal (car svex) 'sv::unfloat)
-                     (equal-len (cdr svex) 1))
-         (all-xor/and/or-nodes-are-masked-p (first (cdr svex)) size env))
-        (t t))))
+;; (bitand/or/xor-cancel-repeated '(sv::Bitand (sv::Bitand a b)
+;;                                            (sv::bitand (sv::bitor a x) y)))
+;; returns:
+;; (BITAND (BITAND A B) Y)
 
-(defun all-xor/and/or-nodes-are-masked-listp (lst size env)
-  (if (atom lst)
-      (equal lst nil)
-    (and (all-xor/and/or-nodes-are-masked-p (car lst) size env)
-         (all-xor/and/or-nodes-are-masked-listp (cdr lst) size env))))
+;; (bitand/or/xor-cancel-repeated '(sv::Bitor (sv::Bitor a b)
+;;                                           (sv::bitand (sv::bitor a x) y)))
+;; returns:
+;; (SV::BITOR (SV::BITOR A B) (BITAND X Y))
+
+;; (bitand/or/xor-cancel-repeated '(sv::Bitor a (sv::bitxor 1 a)))
+;; returns:
+;; 1
+
+;; (bitand/or/xor-cancel-repeated 'sv::bitand `x `(sv::bitxor x y)
+;;                               :env (make-fast-alist `((x . x) (y . y)))
+;;                               :context `((integerp x) (Integerp y)))
+;; returns
+;; (BITAND X (BITXOR -1 Y))
+;;)
+
+;; (bitand/or/xor-cancel-repeated 'sv::bitxor
+;;                                `(sv::bitxor (sv::bitxor x y) z) `(bitxor a (sv::bitxor x y))
+;;                                :env (make-fast-alist `((x . x) (y . y)))
+;;                                :context `((integerp x) (Integerp y)))
+;; returns
+;; (BITXOR Z A)
+
+;;;;;;;;;;;;;;;;;;;;;;;;;;;;;;;;;;;;;;;;;;;;;;;;;;;;;;;;;;;;;;;;;;;;;;;;;;;
+;; Proofs
+;;;;;;;;;;;;;;;;;;;;;;;;;;;;;;;;;;;;;;;;;;;;;;;;;;;;;;;;;;;;;;;;;;;;;;;;;;;
 
 (local
  (defthm svex-eval-opener-when-call
@@ -322,7 +482,7 @@
             :in-theory (e/d (SV::3VEC-BITOR) ())))))
 
 (Local
- (acl2::defsection single-bit-part-select-case-splitter
+ (defsection single-bit-part-select-case-splitter
 
    (defun single-bit-4vec-p-ored (x)
      (or (equal x 1)
@@ -508,12 +668,7 @@
                              PUSH-3VEC-FIX-INTO-4VEC-PART-SELECT)
                             (4VEC-PART-SELECT-OF-3VEC-FIX
                              ;;
-                             )))
-           #|(and stable-under-simplificationp
-           '(:use ((:instance when-4vec-bitor-is-zero ; ; ;
-           (x (4VEC-PART-SELECT 0 1 (EVAL-BITOR-LST (CDR LEAVES) ENV))) ; ; ;
-           (y (4VEC-PART-SELECT 0 1 (SVEX-EVAL (CAR ; ; ;
-           LEAVES) ENV)))))))|#)))
+                             ))))))
 
 (local
  (defthm when-eval-bitand-lst-evals-to-0
@@ -532,11 +687,7 @@
                              PUSH-3VEC-FIX-INTO-4VEC-PART-SELECT)
                             (4VEC-PART-SELECT-OF-3VEC-FIX
                              ;;
-                             )))
-           #|(and stable-under-simplificationp
-           '(:use ((:instance when-4vec-bitor-is-zero ; ; ;
-           (x (4VEC-PART-SELECT 0 1 (EVAL-BITOR-LST (CDR LEAVES) ENV))) ; ; ;
-           (y (4VEC-PART-SELECT 0 1 (SVEX-EVAL (CAR LEAVES) ENV)))))))|#)))
+                             ))))))
 
 (local
  (defthm svex-eval-when-fnc-is-bitand
@@ -589,16 +740,34 @@
                              SVEX-CALL->FN )
                             ())))))
 
+(local
+ (defthmd svex-eval-of-4vec-p
+   (implies (4vec-p x)
+            (equal (svex-eval x env)
+                   x))
+   :rule-classes :rewrite
+   :hints (("Goal"
+            :in-theory (e/d (svex-eval svex-kind SV::SVEX-QUOTE->VAL svex-p 4vec-p) ())))))
+
+(local
+ (defthmd 4vec-rsh-1-of-single-bit
+   (implies (equal (4vec-part-select 0 1 x) x)
+            (equal (4vec-rsh 1 x) 0))))
+
 (defthm bitand/or/xor-simple-constant-simplify-correct-1
   (implies (and (or (equal fn 'sv::bitor)
                     (equal fn 'sv::bitxor)
                     (equal fn 'sv::bitand)
-                    ))
+                    )
+                (svex-p arg1)
+                (svex-p arg2))
            (equal (svex-eval (bitand/or/xor-simple-constant-simplify fn arg1 arg2 nil)
                              env)
                   (svex-eval `(,fn ,arg1 ,arg2) env)))
   :hints (("goal"
            :in-theory (e/d (svex-apply
+                            4vec-rsh-1-of-single-bit
+                            svex-eval-of-4vec-p
                             bitand/or/xor-simple-constant-simplify) ;
                            ()))))
 
@@ -615,7 +784,8 @@
   :otf-flg t
   :hints (("goal"
            :in-theory (e/d (svex-apply
-
+                            svex-eval-of-4vec-p
+                            and*
                             bitand/or/xor-simple-constant-simplify) ;
                            ()))
           (and stable-under-simplificationp
@@ -673,104 +843,6 @@
                             (rp-trans))))))
 
 (local
- (defthm EVAL-BITAND-LST-when-all-xor/and/or-nodes-are-masked-listp
-   (implies (and (case-split (consp leaves))
-                 (all-xor/and/or-nodes-are-masked-listp leaves 1 env))
-            (equal (4VEC-PART-SELECT 0 1
-                                     (EVAL-BITAND-LST LEAVES env))
-                   (EVAL-BITAND-LST LEAVES env)))
-   :hints (("Goal"
-            :expand ((ALL-XOR/AND/OR-NODES-ARE-MASKED-P (CAR LEAVES)
-                                                        1 ENV))
-            :in-theory (e/d (4VEC-PART-SELECT-OF-4VEC-BITAND-BETTER
-                             )
-                            ())))))
-
-(local
- (defthm all-xor/and/or-nodes-are-masked-listp-of-append
-   (implies (and (all-xor/and/or-nodes-are-masked-listp x size env)
-                 (all-xor/and/or-nodes-are-masked-listp y size env))
-            (all-xor/and/or-nodes-are-masked-listp (append x y) size env))))
-
-(local
- (defret all-xor/and/or-nodes-are-masked-listp-of-<fn>
-   (implies (and (all-xor/and/or-nodes-are-masked-p svex size env)
-                 (or (equal fn 'sv::bitor)
-                     (equal fn 'sv::bitand)
-                     (equal fn 'sv::bitxor)))
-            (all-xor/and/or-nodes-are-masked-listp
-             leaves size env))
-   :fn bitand/bitor-collect-leaves
-   :hints (("goal"
-            :in-theory (e/d (bitand/bitor-collect-leaves
-                             equal-len
-                             all-xor/and/or-nodes-are-masked-p) ())))))
-
-(local
- (defthm all-xor/and/or-nodes-are-masked-p-implies
-   (implies (all-xor/and/or-nodes-are-masked-p svex size env)
-            (equal (4vec-part-select 0 size (svex-eval svex env))
-                   (svex-eval svex env)))
-   :rule-classes :forward-chaining
-   :hints (("goal"
-            :in-theory (e/d (all-xor/and/or-nodes-are-masked-p) ())))))
-
-(local
- (defthm all-xor/and/or-nodes-are-masked-p-implies-2
-   (implies (and (all-xor/and/or-nodes-are-masked-p svex size env)
-                 (equal (car svex) 'sv::unfloat)
-                 (consp (cdr svex))
-                 (atom (cddr svex))
-                 (not (cddr svex)))
-            (and #|(equal (4vec-part-select 0 size (svex-eval (cadr svex) env))
-             (svex-eval (cadr svex) env))|#
-             (all-xor/and/or-nodes-are-masked-p (cadr svex)
-                                                size env)))
-   :rule-classes :forward-chaining
-   :hints (("goal"
-
-            :expand ((svex-eval svex env)
-                     (all-xor/and/or-nodes-are-masked-p svex size env))
-            :in-theory (e/d (svex-call->fn
-                             svex-kind
-                             equal-len
-                             svex-apply
-                             svexlist-eval
-                             svex-call->args
-                             all-xor/and/or-nodes-are-masked-p)
-                            ())))))
-
-(local
- (defret all-xor/and/or-nodes-are-masked-p-of-<fn>
-   (implies (and (or (and (or (equal fn 'sv::bitxor)
-                              (equal fn 'sv::bitor)
-                              (equal fn 'sv::bitand))
-                          (equal-len args 2))
-                     (and (equal fn 'sv::unfloat)
-                          (equal-len args 1)))
-                 (natp size)
-                 (all-xor/and/or-nodes-are-masked-listp args size env))
-            (all-xor/and/or-nodes-are-masked-p res size env))
-   :fn svex-reduce-w/-env-apply-specials
-   :hints (("Goal"
-            :expand ((ALL-XOR/AND/OR-NODES-ARE-MASKED-LISTP ARGS SIZE ENV)
-                     (ALL-XOR/AND/OR-NODES-ARE-MASKED-LISTP (CDR ARGS)
-                                                            SIZE ENV)
-                     (:free (fn args)
-                            (ALL-XOR/AND/OR-NODES-ARE-MASKED-P (cons fn args)
-                                                               size env)))
-            :in-theory (e/d (ALL-XOR/AND/OR-NODES-ARE-MASKED-LISTP
-                             SVEX-APPLY
-                             equal-len
-                             SVEXLIST-EVAL
-                             4VEC-PART-SELECT-OF-4VEC-BITXOR-BETTER
-                             4VEC-PART-SELECT-OF-4VEC-BITor-better
-                             4VEC-PART-SELECT-OF-4VEC-BITand-better
-                             ;;all-xor/and/or-nodes-are-masked-p
-                             SVEX-REDUCE-W/-ENV-APPLY-SPECIALS)
-                            ())))))
-
-(local
  (defthmd svex-eval-of-4vec
    (implies (4vec-p x)
             (equal (svex-eval x a)
@@ -782,113 +854,50 @@
                              svex-kind)
                             ())))))
 
-(defret all-xor/and/or-nodes-are-masked-p-of-<fn>
-  (implies (and (or (and (or (equal fn 'sv::bitxor)
-                             (equal fn 'sv::bitor)
-                             (equal fn 'sv::bitand))
-                         (equal-len args 2))
-                    (and (equal fn 'sv::unfloat)
-                         (equal-len args 1)))
-                (natp size)
-                (all-xor/and/or-nodes-are-masked-listp args size env))
-           (all-xor/and/or-nodes-are-masked-p res size env))
-  :fn svex-reduce-w/-env-apply
-  :hints (("goal"
+(progn
+  (local
+   (defthm 4vec-bitxor-of-two-ones
+     (equal (SV::4VEC-BITXOR x (SV::4VEC-BITXOR 1 1))
+            (sv::3vec-fix x))
+     :hints (("Goal"
+              :in-theory (e/d ()
+                              (4vec)))
+             )))
 
-           :expand ((all-xor/and/or-nodes-are-masked-p (sv::4vec-bitxor (car args) (cadr args))
-                                                       size env)
-                    (all-xor/and/or-nodes-are-masked-p (4vec-bitand (car args) (cadr args))
-                                                       size env)
-                    (all-xor/and/or-nodes-are-masked-p (4vec-bitor (car args) (cadr args))
-                                                       size env)
-                    (all-xor/and/or-nodes-are-masked-p (car args)
-                                                       size env)
-                    (all-xor/and/or-nodes-are-masked-p (cadr args)
-                                                       size env)
-                    (all-xor/and/or-nodes-are-masked-p (sv::3vec-fix (car args))
-                                                       size env)
-                    (all-xor/and/or-nodes-are-masked-listp args size env))
-           :in-theory (e/d (svex-eval-of-4vec
-                            all-xor/and/or-nodes-are-masked-listp
-                            all-xor/and/or-nodes-are-masked-p
-                            svex-apply
-                            equal-len
-                            svexlist-eval
-                            4vec-part-select-of-4vec-bitxor-better
-                            4vec-part-select-of-4vec-bitor-better
-                            4vec-part-select-of-4vec-bitand-better
-                            ;;all-xor/and/or-nodes-are-masked-p
-                            svex-reduce-w/-env-apply)
-                           ()))))
+  (local
+   (defthm 4vec-bitxor-of-two-ones-2
+     (equal (SV::4VEC-BITXOR 1 (SV::4VEC-BITXOR 1 x))
+            (sv::3vec-fix x))
+     :hints (("Goal"
+              :use ((:instance 4vec-bitxor-of-two-ones))
+              :in-theory (e/d ()
+                              (4vec-bitxor-of-two-ones
+                               (:e sv::4vec-bitxor)
+                               4vec)))
+             )))
 
-(defret all-xor/and/or-nodes-are-masked-p-of-<fn>
-  (implies (and (natp size)
-                (all-xor/and/or-nodes-are-masked-p arg1 size env)
-                (all-xor/and/or-nodes-are-masked-p arg2 size env)
-                (or (equal fn 'sv::bitxor)
-                    (equal fn 'sv::bitor)
-                    (equal fn 'sv::bitand)))
-           (all-xor/and/or-nodes-are-masked-p simplified-svex size env))
-  :fn bitand/or/xor-simple-constant-simplify
-  ;;:otf-flg t
-  :hints (("Goal"
-           :expand ((ALL-XOR/AND/OR-NODES-ARE-MASKED-P (4VEC-BITAND ARG1 ARG2)
-                                                       SIZE ENV)
-                    (ALL-XOR/AND/OR-NODES-ARE-MASKED-P (SV::4VEC-BITXOR ARG1 ARG2)
-                                                       SIZE ENV)
-                    (ALL-XOR/AND/OR-NODES-ARE-MASKED-P (4VEC-BITOR ARG1 ARG2)
-                                                       SIZE ENV)
-                    (ALL-XOR/AND/OR-NODES-ARE-MASKED-P ARG1 SIZE ENV)
-                    (ALL-XOR/AND/OR-NODES-ARE-MASKED-P ARG2 SIZE ENV)
-                    (ALL-XOR/AND/OR-NODES-ARE-MASKED-P (SV::3VEC-FIX ARG1)
-                                                       SIZE ENV)
-                    (ALL-XOR/AND/OR-NODES-ARE-MASKED-P (SV::3VEC-FIX ARG2)
-                                                       SIZE ENV))
-           :do-not-induct t
-           :in-theory (e/d (svex-eval-of-4vec
-                            equal-len
-                            4VEC-PART-SELECT-OF-4VEC-BITXOR-BETTER
-                            4VEC-PART-SELECT-OF-4VEC-BITor-better
-                            4VEC-PART-SELECT-OF-4VEC-BITand-better
-                            ;;SVEX-REDUCE-W/-ENV-APPLY
-                            ;;SVEX-REDUCE-W/-ENV-APPLY-SPECIALS
-                            SVEX-APPLY
-                            4VEC-PART-SELECT-OF-3VEC-FIX
-                            all-xor/and/or-nodes-are-masked-p
-                            bitand/or/xor-simple-constant-simplify)
-                           ()))))
+  (local
+   (defthm clear-1s-from-bitxor-correct-lemma
+     (IMPLIES (AND (BITXOR-HAS-1 x)
+                   (svex-p x))
+              (EQUAL (svex-eval (remove-1-from-xor x) ENV)
 
-(local
- (defret all-xor/and/or-nodes-are-masked-p-of-<fn>
-   (implies (and (force (natp size))
-                 (all-xor/and/or-nodes-are-masked-p svex size env2)
-                 (all-xor/and/or-nodes-are-masked-p new-val size env2))
-            (all-xor/and/or-nodes-are-masked-p simplified-svex size env2))
-   :fn BITAND/BITOR-CANCEL-REPEATED-AUX
-   :hints (("Goal"
-            :do-not-induct t
-            :induct (BITAND/BITOR-CANCEL-REPEATED-AUX svex
-                                                      leaves new-val
-                                                      :limit limit
-                                                      )
-            ;;:induct (all-xor/and/or-nodes-are-masked-p svex size env)
-            :expand ((bitand/bitor-cancel-repeated-aux SVEX LEAVES NEW-VAL
-                                                       :LIMIT LIMIT))
-            :in-theory (e/d (4VEC-PART-SELECT-OF-4VEC-BITXOR-BETTER
-                             equal-len acl2::and*
-                             4VEC-PART-SELECT-OF-4VEC-BITor-better
-                             4VEC-PART-SELECT-OF-4VEC-BITand-better
-                             all-xor/and/or-nodes-are-masked-p
-                             bitand/bitor-cancel-repeated-aux)
-                            ())))))
+                     (sv::4vec-bitxor 1
+                                      (SVEX-EVAL x env))))
+     :hints (("Goal"
+              :in-theory (e/d (BITXOR-HAS-1
+                               SVEX-APPLY
+                               REMOVE-1-FROM-XOR)
+                              ())))))
 
-(defthm all-xor/and/or-nodes-are-masked-p-implies-single-bit-4vec-p
-  (implies (all-xor/and/or-nodes-are-masked-p svex 1 env)
-           (SINGLE-BIT-4VEC-P (svex-eval svex env)))
-  :hints (("Goal"
-           :do-not-induct t
-           :expand ((all-xor/and/or-nodes-are-masked-p svex 1 env))
-           :in-theory (e/d () ()))))
+  (local
+   (defret clear-1s-from-bitxor-correct
+     (implies (svex-p x)
+              (equal (svex-eval res env)
+                     (svex-eval x env)))
+     :fn clear-1s-from-bitxor
+     :hints (("goal"
+              :in-theory (e/d (clear-1s-from-bitxor) ()))))))
 
 (local
  (defret bitand/bitor-cancel-repeated-aux-correct-1
@@ -899,11 +908,6 @@
                  (rp::rp-term-listp context)
                  (rp::eval-and-all context a)
                  (rp::falist-consistent-aux env env-term)
-
-                 (or (equal 1masked nil)
-                     (and (equal 1masked t)
-                          (ALL-XOR/AND/OR-NODES-ARE-MASKED-P svex 1 (rp-evlt env-term a))
-                          (all-xor/and/or-nodes-are-masked-listp leaves 1 (rp-evlt env-term a))))
                  )
             (equal
              (4vec-bitor (eval-bitor-lst leaves (rp-evlt env-term a))
@@ -912,56 +916,124 @@
                          (svex-eval svex (rp-evlt env-term a)))))
    :fn bitand/bitor-cancel-repeated-aux
    ;;:otf-flg t
-   :hints (("Goal"
+   :hints (("Goal" 
             :induct (bitand/bitor-cancel-repeated-aux svex leaves  new-val :limit limit)
             :do-not-induct t
-            :expand (;;(SVEX-EVAL SVEX ENV)
+            :expand ((:free (x)
+                            (svex-apply 'sv::bitxor x))
                      (:free (x)
-                            (SVEX-APPLY 'sv::bitxor x))
+                            (svex-apply 'sv::unfloat x))
                      (:free (x)
-                            (SVEX-APPLY 'sv::unfloat x))
+                            (svex-apply 'sv::bitand x))
                      (:free (x)
-                            (SVEX-APPLY 'sv::bitand x))
-                     (:free (x)
-                            (SVEX-APPLY 'sv::bitor x)))
+                            (svex-apply 'sv::bitor x)))
 
-            :in-theory (e/d (ALL-XOR/AND/OR-NODES-ARE-MASKED-P
-                             sv::Svex-p
-                             SVEXLIST-EVAL
+            :in-theory (e/d (;;all-xor/and/or-nodes-are-masked-p
+                             sv::svex-p
+                             svexlist-eval
                              4vec-bitor-of-4vec-bitand
-                             4VEC-PART-SELECT-OF-4VEC-BITOR-BETTER
-                             4VEC-PART-SELECT-OF-4VEC-BITXOR-BETTER
-                             4VEC-PART-SELECT-OF-4VEC-BITAND-BETTER
-                             ;;SVEX-EVAL
-                             SVEX-KIND
-                             SVEX-CALL->FN
-                             SVEX-CALL->ARGS
+                             4vec-part-select-of-4vec-bitor-better
+                             4vec-part-select-of-4vec-bitxor-better
+                             4vec-part-select-of-4vec-bitand-better
+                             ;;svex-eval
+                             svex-kind
+                             svex-call->fn
+                             svex-call->args
                              bitand/bitor-cancel-repeated-aux
                              )
-                            (PUSH-3VEC-FIX-INTO-4VEC-PART-SELECT
-                             SINGLE-BIT-4VEC-P
-                             ;;4VEC-PART-SELECT-OF-3VEC-FIX
+                            (push-3vec-fix-into-4vec-part-select
+                             single-bit-4vec-p
                              member-equal
-                             ;;SVEX-EVAL-WHEN-4VEC-P
-                             DEFAULT-CAR
-                             SV::SVEX-EVAL-WHEN-QUOTE
-                             SV::SVEX-EVAL-WHEN-FNCALL
-                             SV::4VEC-P-WHEN-MAYBE-4VEC-P
-                             (:REWRITE-QUOTED-CONSTANT  SV::SVEX-FIX-UNDER-SVEX-EQUIV)
+                             default-car
+                             sv::svex-eval-when-quote
+                             sv::svex-eval-when-fncall
+                             sv::4vec-p-when-maybe-4vec-p
+                             (:rewrite-quoted-constant  sv::svex-fix-under-svex-equiv)
                              (:definition true-list-listp)
-                             (:rewrite
-                              acl2::member-equal-newvar-components-1)
-                             ;;single-bit-4vec-p-ored-of-4vec-part-select-0-1
+                             (:rewrite acl2::member-equal-newvar-components-1)
                              )))
            (and stable-under-simplificationp
                 '(:clause-processor
                   (single-bit-part-select-case-splitter clause)))
            )))
 
-(Local
+(local
+ (encapsulate
+   nil
+   (local
+    (use-equal-by-logbitp t))
+
+   (local
+    (in-theory (enable acl2::b-and
+                       acl2::b-ior)))
+
+   (local
+    (defthmd logand-of-single-loghead-2
+      (and (equal (logand x (loghead size y))
+                  (loghead size (logand x y)))
+           (equal (logand (loghead size y) x)
+                  (loghead size (logand x y))))
+      :hints (("goal"
+               :use ((:instance logand-of-single-loghead))
+               :in-theory (e/d* (bitops::ihsext-recursive-redefs
+                                 bitops::ihsext-inductions)
+                                ()) ))))
+
+   (defthmd pull-out-part-select-from-4vec-bitand
+     (implies (natp width)
+              (equal (4vec-bitand x
+                                  (4vec-part-select 0 width y))
+                     (4vec-part-select 0 width
+                                       (4vec-bitand x y))))
+     :hints (("goal"
+              :in-theory (e/d (4vec-bitand
+                               3vec-bitand
+                               4vec-part-select
+                               4vec-concat
+                               4vec
+                               sv::3vec-fix)
+                              (4vec
+                               logapp logand loghead
+                               )))
+             (bitops::logbitp-reasoning)
+             ))
+
+   (defthmd move-over-part-select-from-4vec-bitand
+     (implies (natp width)
+              (equal (4vec-bitand x
+                                  (4vec-part-select 0 width y))
+                     (4vec-bitand y
+                                  (4vec-part-select 0 width x))))
+     :hints (("goal"
+              :in-theory (e/d (4vec-bitand
+                               3vec-bitand
+                               4vec-part-select
+                               4vec-concat
+                               4vec
+                               sv::3vec-fix)
+                              (4vec
+                               logapp logand loghead
+                               )))
+             (bitops::logbitp-reasoning)
+             ))
+
+   (defthm width-of-eval-bitand-lst-lemma
+     (implies (and (member-equal svex leaves)
+                   (natp width)
+                   (equal (4vec-part-select 0 width (svex-eval svex env))
+                          (svex-eval svex env)))
+              (equal (4vec-part-select 0 width (eval-bitand-lst leaves env))
+                     (eval-bitand-lst leaves env)))
+     :hints (("goal"
+              :in-theory (e/d (move-over-part-select-from-4vec-bitand
+                               member-equal
+                               eval-bitand-lst
+                               4vec-part-select-of-4vec-bitand-better)
+                              ()))))))
+
+(local
  (defret bitand/bitor-cancel-repeated-aux-correct-2
    (implies (and (equal new-val -1)
-                 (equal 1masked nil)
                  (svexlist-p leaves)
                  (sv::svex-p svex)
                  (rp::rp-term-listp context)
@@ -973,112 +1045,42 @@
              (4vec-bitand (eval-bitand-lst leaves (rp-evlt env-term a))
                           (svex-eval svex (rp-evlt env-term a)))))
    :fn bitand/bitor-cancel-repeated-aux
-   ;;:otf-flg t
-   :hints (("Goal"
+   :otf-flg t
+   :hints (("goal"
             :induct (bitand/bitor-cancel-repeated-aux svex leaves  new-val :limit limit)
             :do-not-induct t
-            :expand (;;(SVEX-EVAL SVEX ENV)
+            :expand (;;(svex-eval svex env)
                      (:free (x)
-                            (SVEX-APPLY 'sv::bitxor x))
+                            (svex-apply 'sv::bitxor x))
                      (:free (x)
-                            (SVEX-APPLY 'sv::unfloat x))
+                            (svex-apply 'sv::unfloat x))
                      (:free (x)
-                            (SVEX-APPLY 'sv::bitand x))
+                            (svex-apply 'sv::bitand x))
                      (:free (x)
-                            (SVEX-APPLY 'sv::bitor x)))
+                            (svex-apply 'sv::bitor x)))
 
-            :in-theory (e/d (sv::Svex-p
-                             SVEXLIST-EVAL
+            :in-theory (e/d (move-over-part-select-from-4vec-bitand
+                             sv::svex-p
+                             svexlist-eval
+                             svex-eval-of-4vec
                              4vec-bitand-of-4vec-bitor
-                             4VEC-PART-SELECT-OF-4VEC-BITOR-BETTER
-                             4VEC-PART-SELECT-OF-4VEC-BITXOR-BETTER
-                             4VEC-PART-SELECT-OF-4VEC-BITAND-BETTER
-                             ;;SVEX-EVAL
-                             SVEX-KIND
-                             SVEX-CALL->FN
-                             SVEX-CALL->ARGS
+                             4vec-part-select-of-4vec-bitor-better
+                             4vec-part-select-of-4vec-bitxor-better
+                             4vec-part-select-of-4vec-bitand-better
+                             svex-kind
+                             svex-call->fn
+                             svex-call->args
                              bitand/bitor-cancel-repeated-aux
                              )
                             (push-3vec-fix-into-4vec-part-select
                              member-equal
-                             ;;SVEX-EVAL-WHEN-4VEC-P
-                             DEFAULT-CAR
-                             SV::SVEX-EVAL-WHEN-QUOTE
-                             SV::SVEX-EVAL-WHEN-FNCALL
-                             SV::4VEC-P-WHEN-MAYBE-4VEC-P
-                             (:REWRITE-QUOTED-CONSTANT  SV::SVEX-FIX-UNDER-SVEX-EQUIV)
+                             default-car
+                             sv::svex-eval-when-quote
+                             sv::svex-eval-when-fncall
+                             sv::4vec-p-when-maybe-4vec-p
+                             (:rewrite-quoted-constant  sv::svex-fix-under-svex-equiv)
                              (:definition true-list-listp)
-                             (:rewrite
-                              acl2::member-equal-newvar-components-1)
-                             ;;single-bit-4vec-p-ored-of-4vec-part-select-0-1
-                             )))
-           (and stable-under-simplificationp
-                '(:clause-processor
-                  (single-bit-part-select-case-splitter clause)))
-           )))
-
-(Local
- (defret bitand/bitor-cancel-repeated-aux-correct-3
-   (implies (and (equal new-val 1)
-                 (svexlist-p leaves)
-                 (sv::svex-p svex)
-                 (rp::rp-term-listp context)
-                 (rp::eval-and-all context a)
-                 (rp::falist-consistent-aux env env-term)
-                 (ALL-XOR/AND/OR-NODES-ARE-MASKED-P svex 1 (rp-evlt env-term a))
-                 (equal 1masked t)
-                 (all-xor/and/or-nodes-are-masked-listp leaves 1 (rp-evlt env-term a))
-                 )
-            (equal
-             (4vec-bitand (eval-bitand-lst leaves (rp-evlt env-term a))
-                          (svex-eval simplified-svex (rp-evlt env-term a)))
-             (4vec-bitand (eval-bitand-lst leaves (rp-evlt env-term a))
-                          (svex-eval svex (rp-evlt env-term a)))))
-   :fn bitand/bitor-cancel-repeated-aux
-   ;;:otf-flg t
-   :hints (("Goal"
-            :induct (bitand/bitor-cancel-repeated-aux svex leaves  new-val :limit limit)
-            :do-not-induct t
-            :expand ((MEMBER-EQUAL SVEX NIL)
-                     ;;(SVEX-EVAL SVEX ENV)
-                     (:free (x)
-                            (SVEX-APPLY 'sv::bitxor x))
-                     (:free (x)
-                            (SVEX-APPLY 'sv::unfloat x))
-                     (:free (x)
-                            (SVEX-APPLY 'sv::bitand x))
-                     (:free (x)
-                            (SVEX-APPLY 'sv::bitor x)))
-
-            :in-theory (e/d (ALL-XOR/AND/OR-NODES-ARE-MASKED-P
-                             SVEXLIST-EVAL
-                             4vec-bitand-of-4vec-bitor
-                             4VEC-PART-SELECT-OF-4VEC-BITOR-BETTER
-                             4VEC-PART-SELECT-OF-4VEC-BITXOR-BETTER
-                             4VEC-PART-SELECT-OF-4VEC-BITAND-BETTER
-                             ;;SVEX-EVAL
-                             SVEX-KIND
-                             SVEX-CALL->FN
-                             SVEX-CALL->ARGS
-                             bitand/bitor-cancel-repeated-aux
-                             )
-                            (push-3vec-fix-into-4vec-part-select
-                             member-equal
-                             ;;SVEX-EVAL-WHEN-4VEC-P
-                             DEFAULT-CAR
-                             SV::SVEX-EVAL-WHEN-QUOTE
-                             SV::SVEX-EVAL-WHEN-FNCALL
-                             SV::4VEC-P-WHEN-MAYBE-4VEC-P
-                             (:REWRITE-QUOTED-CONSTANT  SV::SVEX-FIX-UNDER-SVEX-EQUIV)
-                             (:definition true-list-listp)
-                             (:rewrite
-                              acl2::member-equal-newvar-components-1)
-                             ;;single-bit-4vec-p-ored-of-4vec-part-select-0-1
-                             )))
-           (and stable-under-simplificationp
-                '(:clause-processor
-                  (single-bit-part-select-case-splitter clause)))
-           )))
+                             acl2::member-equal-newvar-components-1))))))
 
 (local
  (defthm eval-bitor/bitand-lst-of-append
@@ -1098,270 +1100,167 @@
                              eval-bitand-lst) ())))))
 
 (local
- (defthm eval-bitor-lst-of-bitand/bitor-collect-leaves
+ (defthm eval-bitor-lst-of-bitand/or/xor-collect-leaves
    (and
     (equal
-     (sv::3vec-fix (eval-bitor-lst (bitand/bitor-collect-leaves svex 'sv::bitor) env))
+     (sv::3vec-fix (eval-bitor-lst (bitand/or/xor-collect-leaves svex 'sv::bitor) env))
      (sv::3vec-fix (svex-eval svex env))))
    :hints (("goal"
             :in-theory (e/d (eval-bitor-lst
                              eval-bitand-lst
-                             bitand/bitor-collect-leaves
+                             bitand/or/xor-collect-leaves
 
                              )
                             ())))))
 
 (local
- (defthm eval-bitand-lst-of-bitand/bitor-collect-leaves
+ (defthm eval-bitand-lst-of-bitand/or/xor-collect-leaves
    (equal
-    (sv::3vec-fix (eval-bitand-lst (bitand/bitor-collect-leaves svex 'sv::bitand) env))
+    (sv::3vec-fix (eval-bitand-lst (bitand/or/xor-collect-leaves svex 'sv::bitand) env))
     (sv::3vec-fix (svex-eval svex env)))
    :hints (("goal"
             :in-theory (e/d (eval-bitor-lst
                              eval-bitand-lst
-                             bitand/bitor-collect-leaves)
+                             bitand/or/xor-collect-leaves)
                             ())))))
 (local
- (defthm eval-bitor-lst-of-bitand/bitor-collect-leaves-2
+ (defthm eval-bitor-lst-of-bitand/or/xor-collect-leaves-2
    (and (equal
          (sv::4vec-bitor other
-                         (eval-bitor-lst (bitand/bitor-collect-leaves svex 'sv::bitor) env)
+                         (eval-bitor-lst (bitand/or/xor-collect-leaves svex 'sv::bitor) env)
                          )
          (sv::4vec-bitor (svex-eval svex env)
                          other))
         (equal
-         (sv::4vec-bitor (eval-bitor-lst (bitand/bitor-collect-leaves svex 'sv::bitor) env)
+         (sv::4vec-bitor (eval-bitor-lst (bitand/or/xor-collect-leaves svex 'sv::bitor) env)
                          other)
          (sv::4vec-bitor (svex-eval svex env)
                          other)))
    :hints (("goal"
-            :use ((:instance eval-bitor-lst-of-bitand/bitor-collect-leaves))
+            :use ((:instance eval-bitor-lst-of-bitand/or/xor-collect-leaves))
             :in-theory (e/d ()
-                            (eval-bitor-lst-of-bitand/bitor-collect-leaves))))))
+                            (eval-bitor-lst-of-bitand/or/xor-collect-leaves))))))
 
 (local
- (defthm eval-bitand-lst-of-bitand/bitor-collect-leaves-2
+ (defthm eval-bitand-lst-of-bitand/or/xor-collect-leaves-2
    (and (equal
          (sv::4vec-bitand other
-                          (eval-bitand-lst (bitand/bitor-collect-leaves svex 'sv::bitand) env)
+                          (eval-bitand-lst (bitand/or/xor-collect-leaves svex 'sv::bitand) env)
                           )
          (sv::4vec-bitand (svex-eval svex env)
                           other))
         (equal
-         (sv::4vec-bitand (eval-bitand-lst (bitand/bitor-collect-leaves svex 'sv::bitand) env)
+         (sv::4vec-bitand (eval-bitand-lst (bitand/or/xor-collect-leaves svex 'sv::bitand) env)
                           other)
          (sv::4vec-bitand (svex-eval svex env)
                           other)))
    :hints (("goal"
-            :use ((:instance eval-bitand-lst-of-bitand/bitor-collect-leaves))
+            :use ((:instance eval-bitand-lst-of-bitand/or/xor-collect-leaves))
             :in-theory (e/d ()
-                            (eval-bitand-lst-of-bitand/bitor-collect-leaves))))))
+                            (eval-bitand-lst-of-bitand/or/xor-collect-leaves))))))
 
 (local
  (defthm 4vec-p-of-EVAL-BITOR/and-LST
    (and (sv::4vec-p (EVAL-BITOR-LST lst env))
         (sv::4vec-p (EVAL-BITand-LST lst env)))))
 
-(defret bitand/bitor-cancel-repeated-correct
+(local
+ (defret bitxor-remove-node-correct
+   (implies (and (svex-p svex)
+                 (integerp (svex-eval node-to-remove env))
+                 success)
+            (equal (svex-eval res-svex env)
+                   (sv::4vec-bitxor (svex-eval node-to-remove env)
+                                    (svex-eval svex env))))
+   :fn bitxor-remove-node
+   :hints (("Goal"
+            :in-theory (e/d (SVEX-P
+                             bitxor-remove-node) ())))))
+
+(local
+ (defret bitxor-remove-nodes-from-both-correct
+   (implies (and (svex-p svex1)
+                 (svex-p svex2)
+                 (svexlist-p nodes-to-remove)
+
+                 (rp::rp-term-listp context)
+                 (rp::eval-and-all context a)
+                 (rp::falist-consistent-aux env env-term)
+                 )
+            (equal (sv::4vec-bitxor (svex-eval res-svex1 (rp-evlt env-term a))
+                                    (svex-eval res-svex2 (rp-evlt env-term a)))
+                   (sv::4vec-bitxor (svex-eval svex1 (rp-evlt env-term a))
+                                    (svex-eval svex2 (rp-evlt env-term a)))))
+   :fn bitxor-remove-nodes-from-both
+   :hints (("Goal"
+            :in-theory (e/d (svex-p
+                             bitxor-remove-nodes-from-both)
+                            ())))))
+
+(defret bitand/or/xor-cancel-repeated-correct
   (implies (and (fnsym-p fn)
                 (sv::svex-p x)
                 (sv::svex-p y)
                 (rp::rp-term-listp context)
                 (rp::eval-and-all context a)
-                (rp::falist-consistent-aux env env-term)
-                (or (equal 1masked nil)
-                    (and (equal 1masked t)
-                         (all-xor/and/or-nodes-are-masked-p x 1 (rp-evlt env-term a))
-                         (all-xor/and/or-nodes-are-masked-p y 1 (rp-evlt env-term a))))
-                )
+                (rp::falist-consistent-aux env env-term))
            (equal
             (svex-eval simplified-svex (rp-evlt env-term a))
             (svex-eval `(,fn ,x ,y) (rp-evlt env-term a))))
-  :fn bitand/bitor-cancel-repeated
+  :fn bitand/or/xor-cancel-repeated
   ;;:otf-flg t
   :hints (("goal"
            :do-not-induct t
            :use ( (:instance bitand/bitor-cancel-repeated-aux-correct-1
                              (svex y)
-                             (leaves (bitand/bitor-collect-leaves x 'bitor))
+                             (leaves (bitand/or/xor-collect-leaves x 'bitor))
 
                              (new-val 0)
+                             (under-xor nil)
                              (limit *bitand/bitor-cancel-repeated-aux-limit*))
                   (:instance bitand/bitor-cancel-repeated-aux-correct-1
                              (svex x)
-                             (leaves (bitand/bitor-collect-leaves
+                             (leaves (bitand/or/xor-collect-leaves
                                       (mv-nth 0
                                               (bitand/bitor-cancel-repeated-aux
                                                y
-                                               (bitand/bitor-collect-leaves x
-                                                                            'bitor)
-                                               0))
+                                               (bitand/or/xor-collect-leaves x
+                                                                             'bitor)
+                                               0
+                                               :under-xor nil))
                                       'bitor))
                              (new-val 0)
+                             (under-xor nil)
                              (limit *bitand/bitor-cancel-repeated-aux-limit*))
                   (:instance bitand/bitor-cancel-repeated-aux-correct-2
                              (svex y)
-                             (leaves (bitand/bitor-collect-leaves x
-                                                                  'bitand))
+                             (leaves (bitand/or/xor-collect-leaves x
+                                                                   'bitand))
 
                              (new-val -1)
+                             (under-xor nil)
                              (limit *bitand/bitor-cancel-repeated-aux-limit*))
                   (:instance bitand/bitor-cancel-repeated-aux-correct-2
                              (svex x)
-                             (leaves (bitand/bitor-collect-leaves
+                             (leaves (bitand/or/xor-collect-leaves
                                       (mv-nth 0
                                               (bitand/bitor-cancel-repeated-aux
                                                y
-                                               (bitand/bitor-collect-leaves x
-                                                                            'bitand)
-                                               -1))
+                                               (bitand/or/xor-collect-leaves x
+                                                                             'bitand)
+                                               -1
+                                               :under-xor nil))
                                       'bitand))
 
                              (new-val -1)
+                             (under-xor nil)
                              (limit *bitand/bitor-cancel-repeated-aux-limit*))
 
-                  (:instance bitand/bitor-cancel-repeated-aux-correct-3
-                             (svex y)
-                             (leaves (bitand/bitor-collect-leaves x
-                                                                  'bitand))
-
-                             (new-val 1)
-                             (limit *bitand/bitor-cancel-repeated-aux-limit*))
-                  (:instance bitand/bitor-cancel-repeated-aux-correct-3
-                             (svex x)
-                             (leaves (bitand/bitor-collect-leaves
-                                      (mv-nth 0
-                                              (bitand/bitor-cancel-repeated-aux
-                                               y
-                                               (bitand/bitor-collect-leaves x
-                                                                            'bitand)
-                                               1))
-                                      'bitand))
-
-                             (new-val 1)
-                             (limit *bitand/bitor-cancel-repeated-aux-limit*))
                   )
-           :in-theory (e/d (ALL-XOR/AND/OR-NODES-ARE-MASKED-P
-                            bitand/bitor-cancel-repeated
+           :in-theory (e/d (bitand/or/xor-cancel-repeated
                             4vec-part-select-of-4vec-bitor-better
                             4vec-part-select-of-4vec-bitand-better)
-                           (eval-bitor-lst-of-bitand/bitor-collect-leaves
+                           (eval-bitor-lst-of-bitand/or/xor-collect-leaves
                             bitand/bitor-cancel-repeated-aux-correct-1
                             bitand/bitor-cancel-repeated-aux-correct-2
-                            bitand/bitor-cancel-repeated-aux-correct-3
                             )))))
-
-;;;;;;;;;;;;;;;;;;;;;;;;;;;;;;;;;;;;;;;;;;;;;;;;;;;;;;;;;;;;;;;;;;;;;;;;;;;
-;;
-
-#|(define reapply-1mask-to-consts-in-bitxor/or/and (svex)
-:returns (mv (simplified-svex sv::Svex-p
-:hyp (svex-p svex)
-)
-changed)
-:prepwork ((Local
-(defthm 4vec-p-implies-svex-p
-(implies (4vec-p x)
-(svex-p x))
-:hints (("Goal"
-:in-theory (e/d (4vec-p svex-p) ()))))))
-(case-match svex
-(('sv::bitor x y)
-(b* (((mv new-x changed-x)
-(reapply-1mask-to-consts-in-bitxor/or/and x))
-((mv new-y changed-y)
-(reapply-1mask-to-consts-in-bitxor/or/and y)))
-(if (or changed-y changed-x)
-(mv (svex-reduce-w/-env-apply 'sv::bitor (hons-list new-x new-y)) t)
-(mv svex nil))))
-(('sv::bitand x y)
-(b* (((mv new-x changed-x)
-(reapply-1mask-to-consts-in-bitxor/or/and x))
-((mv new-y changed-y)
-(reapply-1mask-to-consts-in-bitxor/or/and y)))
-(if (or changed-y changed-x)
-(mv (svex-reduce-w/-env-apply 'sv::bitand (hons-list new-x new-y)) t)
-(mv svex nil))))
-(('sv::bitxor x y)
-(b* (((mv new-x changed-x)
-(reapply-1mask-to-consts-in-bitxor/or/and x))
-((mv new-y changed-y)
-(reapply-1mask-to-consts-in-bitxor/or/and y)))
-(if (or changed-y changed-x)
-(mv (svex-reduce-w/-env-apply 'sv::bitxor (hons-list new-x new-y)) t)
-(mv svex nil))))
-(&
-(if (4vec-p svex)
-(mv (4vec-part-select 0 1 svex)
-(not (equal (4vec-part-select 0 1 svex) svex)))
-(mv svex nil))))
-
-///
-
-(defret <fn>-is-correct
-(implies (single-bit-4vec-p (svex-eval svex env))
-(equal (svex-eval simplified-svex env)
-(svex-eval svex env)))
-:hints (("Goal"
-:do-not-induct t
-:expand ((:free (x) (SVEX-APPLY 'BITXOR x)))
-:induct (reapply-1mask-to-consts-in-bitxor/or/and svex)
-:in-theory (e/d (SVEXLIST-EVAL
-4VEC-PART-SELECT-OF-4VEC-BITXOR-BETTER
-SVEX-EVAL
-SVEX-KIND
-SVEX-CALL->FN
-SVEX-VAR->NAME
-4vec-p
-SV::SVEX-QUOTE->VAL
-SVEX-CALL->args)
-()))))
-
-)|#
-
-;; (define count-ones-in-bitxor (svex
-;;                               &optional
-;;                               (1masked '1masked))
-;;   :returns (res natp)
-;;   (('sv::bitxor x y)
-;;    (b* (((mv new-x changed-x)
-;;          (count-ones-in-bitxor x ))
-;;         ((mv new-y changed-y)
-;;          (remove-repeated-ones-from-bitxor y)))
-;;      (if (or changed-y changed-x)
-;;          (svex-reduce-w/-env-apply 'sv::bitand (hons-list x y))
-;;        svex)))
-;;   (& (cond ((not (integerp svex))
-;;             0)
-;;            ((not 1masked)
-;;             ;; assuming here that when not 1masked, it can only be simplified when it is
-;;             (equal svex -1))
-;;             ))
-
-;; (define remove-repeated-ones-from-bitxor ((svex) 1masked)
-;;   :returns (mv simplified-svex changed)
-;;   (case-match svex
-;;     (('sv::bitor x y)
-;;      (b* (((mv new-x changed-x)
-;;            (remove-repeated-ones-from-bitxor x))
-;;           ((mv new-y changed-y)
-;;            (remove-repeated-ones-from-bitxor y)))
-;;        (if (or changed-y changed-x)
-;;            (svex-reduce-w/-env-apply 'sv::bitxor (hons-list x y))
-;;          svex)))
-;;     (('sv::bitand x y)
-;;      (b* (((mv new-x changed-x)
-;;            (remove-repeated-ones-from-bitxor x))
-;;           ((mv new-y changed-y)
-;;            (remove-repeated-ones-from-bitxor y)))
-;;        (if (or changed-y changed-x)
-;;            (svex-reduce-w/-env-apply 'sv::bitand (hons-list x y))
-;;          svex)))
-;;     (('sv::bitxor x y)
-;;      (b* (((mv new-x changed-x)
-;;            (remove-repeated-ones-from-bitxor x))
-;;           ((mv new-y changed-y)
-;;            (remove-repeated-ones-from-bitxor y)))
-;;        (if (or changed-y changed-x)
-;;            (svex-reduce-w/-env-apply 'sv::bitand (hons-list x y))
-;;          svex)))
